Phi_System/IDE_CP_App2.thy
@@ -22,7 +22,7 @@ ML_file \<open>library/phi_type_algebra/inhabited_type.ML\<close>
 
 end
 
-\<phi>property_deriver Inhabited_Type 100 for (\<open>Inhabited_Type _\<close>)
+\<phi>property_deriver Inhabited_Type 80 for (\<open>Inhabited_Type _\<close>)
     = \<open> Phi_Type_Derivers.inhabited_type \<close> 
 
 
@@ -45,12 +45,27 @@ private lemma \<phi>TA_SemTy_cong:
 \<Longrightarrow> Weak_Semantic_Type T TY \<equiv> Weak_Semantic_Type T TY' \<close>
   by simp
 
+private lemma Semantic_Type_derv:
+  \<open> (Ant @tag \<phi>TA_ANT \<Longrightarrow> Weak_Semantic_Type T TY)
+\<Longrightarrow> (Ant @tag \<phi>TA_ANT \<Longrightarrow> Inhabited_Type T)
+\<Longrightarrow> \<r>Success
+\<Longrightarrow> \<o>\<b>\<l>\<i>\<g>\<a>\<t>\<i>\<o>\<n> True
+\<Longrightarrow> Ant @tag \<phi>TA_ANT
+\<Longrightarrow> Semantic_Type T TY \<close>
+  unfolding Semantic_Type_def
+  by blast
+
+
 ML_file \<open>library/phi_type_algebra/semantic_type.ML\<close>
 
 end
 
 \<phi>property_deriver Weak_Semantic_Type 100 for (\<open>Weak_Semantic_Type _ _\<close>)
-    = \<open> Phi_Type_Derivers.semantic_type \<close> 
+    = \<open> Phi_Type_Derivers.semantic_type true \<close> 
+
+\<phi>property_deriver Semantic_Type 90 for (\<open>Semantic_Type _ _\<close>)
+  requires Inhabited_Type
+    = \<open> Phi_Type_Derivers.semantic_type false \<close>
 
 
 subsubsection \<open>Semantic Zero Value\<close>
@@ -70,7 +85,7 @@ ML_file \<open>library/phi_type_algebra/semantic_zero_val.ML\<close>
 
 end
 
-\<phi>property_deriver Semantic_Zero_Val 110 for (\<open>Semantic_Zero_Val _ _ _\<close>)
+\<phi>property_deriver Semantic_Zero_Val 120 for (\<open>Semantic_Zero_Val _ _ _\<close>)
   requires Weak_Semantic_Type
     = \<open> Phi_Type_Derivers.semantic_zero_val \<close> 
 
